Fix admits in examples apart from slprop_extensionality

examples/steel/Queue.fsti
@@ -13,8 +13,9 @@ let pts_to (#a:_) (x:t a) ([@@@smt_fallback]v: Ghost.erased (cell a)) = pts_to x
 val queue_l (#a:_) (hd tl:Ghost.erased (t a)) (l:Ghost.erased (list a))
   : vprop
 
-let queue (#a:_) ([@@@smt_fallback] hd:Ghost.erased (t a))
-                 ([@@@smt_fallback] tl:Ghost.erased (t a)) = h_exists (queue_l hd tl)
+val queue (#a:_) ([@@@smt_fallback] hd:Ghost.erased (t a))
+                 ([@@@smt_fallback] tl:Ghost.erased (t a)) : vprop
+                //= h_exists (queue_l hd tl)
 
 val new_queue (#a:_) (v:a) :
   SteelSelT (t a) emp (fun x -> queue x x)
